problems/8/QuickUnion.dfy
@@ -1,0 +1,242 @@
+
+module QuickUnion {
+
+
+    class QuickUnion {
+        var n : nat
+        var parent: array<nat>
+        var size: array<nat>
+
+        constructor(n: nat) 
+            requires n > 0
+            ensures this.n == n
+            ensures this.parent.Length == this.n
+            ensures this.size.Length == this.n
+            ensures fresh(this)
+            ensures Valid()
+        {
+            parent := new nat[n];
+            size := new nat[n];
+            this.n := n;
+            new;
+            assert parent.Length == n;
+            assert size.Length == n;
+            forall i | 0 <= i < n {
+                parent[i] := i;
+            }
+            forall i | 0 <= i < n {
+                size[i] := 1;
+            }
+        }
+
+        predicate Valid()
+            reads this, parent, size
+        {
+            this.parent.Length > 0 &&
+            this.parent.Length == this.size.Length == this.n &&
+            this.parent != this.size &&
+            (forall i :: 0 <= i < this.parent.Length ==> 0 <= parent[i] < parent.Length)
+            && (forall i :: 0 <= i < this.size.Length ==> this.size[i] > 0)
+        }
+
+        method findRoot(x: nat) returns (root: nat)
+            requires Valid()
+            requires 0 <= x < parent.Length
+            ensures 0 <= root < parent.Length
+            ensures parent.Length == old(parent.Length)
+            ensures old(this.n) == this.n
+            ensures Valid()
+            modifies parent
+            decreases *
+        {
+            root := x;
+            // ghost var all := multiset(parent[..]);
+            // ghost var visited: set<nat> := {};
+            while root != parent[root]
+                invariant Valid()
+                invariant 0 <= root < parent.Length
+                decreases *
+            {
+                root := parent[root];
+            }
+            this.parent[x] := root;
+        }
+
+        method connected(x: nat, y: nat) returns (result: bool)
+            requires 0 <= x < parent.Length
+            requires 0 <= y < parent.Length
+            requires Valid()
+            decreases *
+            modifies parent
+            ensures old(this.n) == this.n
+            ensures Valid()
+            ensures fresh(old(this)) ==> fresh(this)
+        {
+            var xroot := this.findRoot(x);
+            var yroot := this.findRoot(y);
+            result := xroot == yroot;
+        }
+
+        method union(x: nat, y: nat)
+            requires 0 <= x < parent.Length
+            requires 0 <= y < parent.Length
+            requires Valid()
+            decreases *
+            modifies parent, size
+            ensures old(this.n) == this.n
+            ensures Valid()
+        {
+            var rootX := findRoot(x);
+            var rootY := findRoot(y);
+            if rootX != rootY {
+                if size[rootX] < size[rootY] {
+                    size[rootY] := size[rootY] + size[rootX];
+                    parent[rootX] := rootY;
+                } else {
+                    size[rootX] := size[rootX] + size[rootY];
+                    parent[rootY] := rootX;
+                }
+            }
+        }
+    }
+
+
+class PriorityQueue<T> {
+  var heap: array<(T, int)>
+  var size: int
+  var capacity: int
+
+  constructor (private_capacity: int, def: T)
+    requires private_capacity > 0 
+    ensures heap.Length == capacity
+    ensures size <= heap.Length
+    ensures size < capacity
+    ensures size == 0
+    ensures fresh(this)
+  {
+    capacity := private_capacity;
+    size := 0;
+    var default := (def, 0);
+    heap := new (T, int)[private_capacity](_ => default);
+  }
+
+  method parent(i: int) returns (p: int)
+    requires 0 <= i < size
+    requires i < heap.Length
+    ensures p < heap.Length
+    ensures i > 0 ==> 0 <= p < size
+    ensures i == 0 ==> p == -1
+  {
+    if i > 0 {
+      p := (i - 1) / 2;
+    } else {
+      p := -1;
+    }
+  }
+
+  method leftChild(i: int) returns (l: int)
+    requires 0 <= i < size
+    ensures l == 2 * i + 1
+  {
+    l := 2 * i + 1;
+  }
+
+  method rightChild(i: int) returns (r: int)
+    requires 0 <= i < size
+    ensures r == 2 * i + 2
+  {
+    r := 2 * i + 2;
+  }
+
+  method swap(i: int, j: int)
+    requires 0 <= i < size && 0 <= j < size
+    requires i < heap.Length && j < heap.Length
+    modifies heap
+    ensures heap[i] == old(heap[j]) && heap[j] == old(heap[i])
+  {
+    var temp := heap[i];
+    heap[i] := heap[j];
+    heap[j] := temp;
+  }
+
+  method heapifyUp(i: int)
+    requires 0 <= i < size
+    requires size <= heap.Length
+    modifies heap
+    decreases i
+  {
+    var current_parent := parent(i);
+
+    if current_parent >= 0 && current_parent < size
+      && 0 <= current_parent < size 
+      && heap[i].1 < heap[current_parent].1
+    {
+      swap(i, current_parent);
+      if (current_parent < i) {
+        heapifyUp(current_parent); 
+      }
+    }
+  }
+
+  method heapifyDown(i: int)
+    requires 0 <= i < size
+    modifies heap
+    decreases size - i
+  {
+    var smallest := i;
+    var left_child := leftChild(i);
+    var right_child := rightChild(i);
+    if left_child < size && left_child < heap.Length && heap[left_child].1 < heap[smallest].1 {
+      smallest := leftChild(i);
+    }
+    if right_child < size && right_child < heap.Length && heap[right_child].1 < heap[smallest].1 {
+      smallest := rightChild(i);
+    }
+    if smallest != i {
+      swap(i, smallest);
+      heapifyDown(smallest);
+    }
+  }
+
+  method insert(item: T, priority: int)
+    requires heap.Length == capacity
+    requires 0 <= size < capacity
+    modifies this, heap
+  {
+    heap[size] := (item, priority);
+    size := size + 1;
+    heapifyUp(size - 1);
+  }
+
+  method extractMin() returns (item: T)
+    requires size > 0
+    requires heap.Length > 0
+    requires size - 1 < heap.Length
+    modifies this, heap
+    ensures size == old(size) - 1
+  {
+    item := heap[0].0;
+    heap[0] := heap[size - 1];
+    size := size - 1;
+    if size > 0 {
+      heapifyDown(0);
+    }
+  }
+
+  // Peek the element with the smallest priority without removing it
+  method peek() returns (item: T)
+    requires size > 0
+    requires heap.Length > 0
+    ensures item == heap[0].0
+  {
+    item := heap[0].0;
+  }
+
+  // Check if the priority queue is empty
+  method isEmpty() returns (empty: bool)
+    ensures empty == (size == 0)
+  {
+    empty := (size == 0);
+  }
+}
+}
